examples/Employee_Model/Design_shallow.thy
@@ -47,8 +47,8 @@ theory
   Design_shallow
 imports
   "../../src/UML_Main"
-  "../../src/compiler/OCL_compiler_static"
-  "../../src/compiler/OCL_compiler_generator_dynamic"
+  "../../src/compiler/Static"
+  "../../src/compiler/Generator_dynamic"
 begin
 
 generation_syntax [ shallow (generation_semantics [ design ])
